extraction/Extr.v
@@ -4,4 +4,5 @@ Extraction Language OCaml.
 Separate Extraction
   EffIR.prog0 EffIR.observe EffIR.run
   Samples.sample_delete Samples.sample_two Samples.sample_ret
-  Samples.sample_neg Samples.sample_nested.
+  Samples.sample_neg Samples.sample_nested
+  Samples.sample_throw Samples.sample_guard5.
